checkpoint

pulse/lib/pulse/core/PulseCore.MemoryAlt.fst
@@ -1592,20 +1592,26 @@ let mem_invariant_eq e m0 m1
   (ensures mem_invariant e m0 == mem_invariant e m1)
 = admit()
 
-#restart-solver
 #push-options "--fuel 0 --ifuel 0 --split_queries no --z3rlimit_factor 2"
+#restart-solver
 let lift_heap_action_aux (#fp:H2.slprop u#a) (#a:Type u#b) (#fp':a -> H2.slprop u#a) (#mut:_)
                      (e:inames)
                      ($f:H2.action #mut #None fp a fp')
 : refined_pre_action (mg_of_mut mut) e (up fp) a (fun x -> up (fp' x))
 = fun (m0:hmem_with_inv_except e (up fp)) ->
     assert (interp (up fp `star` mem_invariant e m0) m0);
+    elim_mem_invariant e m0;
+    assert (heap_ctr_valid m0.ctr m0.ghost_ctr m0.iname_ctr m0.iheap);
     let ih0 = m0.iheap in
     let h0 = m0.iheap.concrete in
     assert (H2.interp fp h0);
     let (| x, h1 |) = f m0.iheap.concrete in
     let ih1 = { m0.iheap with concrete = h1 } in
     let m1 = { m0 with iheap = ih1 } in
+    assume (heap_ctr_valid m1.ctr m1.ghost_ctr m1.iname_ctr m1.iheap);
+    mem_invariant_eq e m0 m1;
+    assume (mem_evolves m0 m1);
+    assume (maybe_ghost_action (mg_of_mut mut) m0 m1);
     let aux (frame:slprop)
     : Lemma 
       (requires
@@ -1660,43 +1666,17 @@ let lift_heap_action_aux (#fp:H2.slprop u#a) (#a:Type u#b) (#fp':a -> H2.slprop 
         returns _
         with _ . (
           assert (pick_frame hr');
-          let ml = { invariants=H0.empty_heap; concrete=hl'} in
+          let ml = { invariants=hl.invariants; concrete=hl'} in
           let mr = {hr with concrete=hr'} in 
           assert ((frame `star` mem_invariant e m0) mr);
           assert ((up (fp' x)) ml);
           assert (idisjoint ml mr);
           assert (H2.join hl' hr' == m1.iheap.concrete);
-          
-          // assert (m1.iheap == ijoin ml mr);
-          admit()
-          // assert (interp ((up (fp' x)) `star` (frame `star` mem_invariant e m0)) m1);
-
-          // assume (mem_evolves m0 m1);
-          // assume (maybe_ghost_action (mg_of_mut mut) m0 m1);
-          // star_assoc (up (fp' x)) frame (mem_invariant e m0);
-          // assume (mem_invariant e m0 == mem_invariant e m1);
-          // admit()
+          assert (m1.iheap == ijoin ml mr);
+          star_assoc (up (fp' x)) frame (mem_invariant e m0);
+          assert (mem_invariant e m0 == mem_invariant e m1)
         )
       )    
-  
-
-      // assert (pick_frame m0.iheap.concrete);
-      // let frm : H2.slprop = H2.as_slprop pick_frame in
-      // eliminate exists hl hr.
-      //     idisjoint hl hr /\
-      //     m0.iheap == ijoin hl hr /\
-      //     up fp hl /\
-      //     (frame `star` mem_invariant e m0) hr
-      // returns H2.interp (fp `H2.star` frm) m0.iheap.concrete
-      // with _ . (
-      //   assert (pick_frame hr.concrete);
-      //   admit();
-      //   H2.intro_star fp frm hl.concrete hr.concrete
-      // );
-
-      // assume (H2.interp (fp `H2.star` frm) m0.iheap.concrete);
-
-      // admit()
     in
     emp_u (up fp);
     emp_u (up (fp' x));
@@ -1718,55 +1698,53 @@ let lift_heap_action_aux (#fp:H2.slprop u#a) (#a:Type u#b) (#fp':a -> H2.slprop 
     // assert (interp ((up fp `star emp) `star` mem_invariant e m0) m0);
     // emp_u (up (fp' x));
     // (| x, m1 |)
-(*)
-    admit() (*)
-    assert (interp (mem_invariant e m0) m0);
+    // assert (interp (mem_invariant e m0) m0);
     
-    elim_mem_invariant e m0;
+    // elim_mem_invariant e m0;
 
 
-    assert (heap_ctr_valid m0.ctr m0.ghost_ctr m0.iname_ctr m0.iheap);
-    let h0 = m0.iheap.concrete in
-    assert (H2.interp fp h0);
-    mem_invariant_is_big e m0;
-    eliminate exists hl hr.
-        idisjoint hl hr /\
-        m0.iheap == ijoin hl hr /\
-        up fp hl /\
-        mem_invariant e m0 hr
-    returns 
-      H2.interp (fp `H2.star` down (mem_invariant e m0)) h0
-    with _ . (
-      assert (up (down (mem_invariant e m0)) == mem_invariant e m0);
-      assert (mem_invariant e m0 { hr with invariants = H0.empty_heap});
-      assert (H2.interp (down (mem_invariant e m0)) hr.concrete);
-      assert (H2.interp fp hl.concrete);
-      assert (H2.disjoint hl.concrete hr.concrete);
-      H2.intro_star fp (down (mem_invariant e m0)) hl.concrete hr.concrete
-    );
-    let (| x, h1 |) = f m0.iheap.concrete in
-    assert (H2.interp (fp' x) h1);
-    let ih1 = { m0.iheap with concrete = h1 } in
-    let m1 = { m0 with iheap = ih1 } in
-    assert (interp (up (fp' x)) m1);
-    assert (H2.is_frame_preserving mut None f);
-    H2.action_framing f (down (mem_invariant e m0)) h0;
-    assert (H2.interp (fp' x `H2.star` down (mem_invariant e m0)) h1);
-    mem_invariant_eq e m0 m1;
-    assert (H2.interp (fp' x `H2.star` down (mem_invariant e m1)) h1);
-    assert  (up (fp' x `H2.star` down (mem_invariant e m1)) m1.iheap);
-    mem_invariant_is_big e m1;
-    assert (interp (up (fp' x) `star` mem_invariant e m1) m1);
-    introduce forall frame.
-      interp ((up fp `star` frame) `star` mem_invariant e m0) m0 ==>
-      interp ((up (fp' x) `star` frame) `star` mem_invariant e m1) m1 /\
-      mem_evolves m0 m1
-    with introduce _ ==> _
-    with _ . (
-      admit()
-    );
-    assert (frame_related_mems (up fp) (up (fp' x)) e m0 m1);
-    (| x, m1 |)
+    // assert (heap_ctr_valid m0.ctr m0.ghost_ctr m0.iname_ctr m0.iheap);
+    // let h0 = m0.iheap.concrete in
+    // assert (H2.interp fp h0);
+    // mem_invariant_is_big e m0;
+    // eliminate exists hl hr.
+    //     idisjoint hl hr /\
+    //     m0.iheap == ijoin hl hr /\
+    //     up fp hl /\
+    //     mem_invariant e m0 hr
+    // returns 
+    //   H2.interp (fp `H2.star` down (mem_invariant e m0)) h0
+    // with _ . (
+    //   assert (up (down (mem_invariant e m0)) == mem_invariant e m0);
+    //   assert (mem_invariant e m0 { hr with invariants = H0.empty_heap});
+    //   assert (H2.interp (down (mem_invariant e m0)) hr.concrete);
+    //   assert (H2.interp fp hl.concrete);
+    //   assert (H2.disjoint hl.concrete hr.concrete);
+    //   H2.intro_star fp (down (mem_invariant e m0)) hl.concrete hr.concrete
+    // );
+    // let (| x, h1 |) = f m0.iheap.concrete in
+    // assert (H2.interp (fp' x) h1);
+    // let ih1 = { m0.iheap with concrete = h1 } in
+    // let m1 = { m0 with iheap = ih1 } in
+    // assert (interp (up (fp' x)) m1);
+    // assert (H2.is_frame_preserving mut None f);
+    // H2.action_framing f (down (mem_invariant e m0)) h0;
+    // assert (H2.interp (fp' x `H2.star` down (mem_invariant e m0)) h1);
+    // mem_invariant_eq e m0 m1;
+    // assert (H2.interp (fp' x `H2.star` down (mem_invariant e m1)) h1);
+    // assert  (up (fp' x `H2.star` down (mem_invariant e m1)) m1.iheap);
+    // mem_invariant_is_big e m1;
+    // assert (interp (up (fp' x) `star` mem_invariant e m1) m1);
+    // introduce forall frame.
+    //   interp ((up fp `star` frame) `star` mem_invariant e m0) m0 ==>
+    //   interp ((up (fp' x) `star` frame) `star` mem_invariant e m1) m1 /\
+    //   mem_evolves m0 m1
+    // with introduce _ ==> _
+    // with _ . (
+    //   admit()
+    // );
+    // assert (frame_related_mems (up fp) (up (fp' x)) e m0 m1);
+    // (| x, m1 |)
 
 // let lift_heap_action_aux (#fp:H2.slprop u#a) (#a:Type u#b) (#fp':a -> H2.slprop u#a) (#mut:_)
 //                      (e:inames)
